changed definition #116 because it was not mono, proof for inner mono done

untimed/NewSpfStep.thy
@@ -19,62 +19,101 @@ lemma sbHdElemWell_inv_ex:"sbHdElemWell sb \<Longrightarrow> \<exists>x. convDis
 
 lemma sbHdElemWell_invConvDiscrUp:"sbHdElemWell sb \<Longrightarrow> \<forall>c\<in>ubDom\<cdot>(sb).((inv convDiscrUp) (sbHdElem\<cdot>sb)) \<rightharpoonup> c = inv Discr (inv Iup ((sbHdElem\<cdot>sb) \<rightharpoonup> c))"
   by (simp add: convDiscrUp_inv_subst sbHdElemWell_def sbHdElem_channel)
+    
+lemma sbHdElem_eq:"\<forall>c\<in>(ubDom\<cdot>sb1). sb1. c \<noteq>\<epsilon> \<Longrightarrow> sb1\<sqsubseteq>sb2 \<Longrightarrow> sbHdElem\<cdot>sb1 = sbHdElem\<cdot>sb2"
+proof
+  fix x::channel
+  assume a1:"\<forall>c\<in>(ubDom\<cdot>sb1). sb1. c \<noteq>\<epsilon>"
+  assume a2:"sb1\<sqsubseteq>sb2"
+  have a3:"ubDom\<cdot>sb1 = ubDom\<cdot>sb2"
+    using a2 ubdom_below by auto
+  show "(sbHdElem\<cdot>sb1) x = (sbHdElem\<cdot>sb2) x"
+    apply(simp add:sbHdElem_def sbHdElem_cont a3)
+    using a1 a2 a3 lshd_eq ubgetch_below by blast
+qed
+  
      
 (* updis bijectiv *)
 thm inv_def
 (* Returns the SPF that switches depending on input.  (spfStep_h1 In Out\<cdot>h)\<cdot>(sbHdElem\<cdot>sb) computes the SPF which has to be applied to the input sb*)
 definition spfStep :: "channel set \<Rightarrow> channel set \<Rightarrow> ('m::message sbElem \<Rightarrow> 'm SPF) \<rightarrow> 'm SPF" where
-"spfStep In Out \<equiv> \<Lambda> h. Abs_ufun (\<Lambda>  sb.  (ubDom\<cdot>sb = In \<and> sbHdElemWell sb) 
-                                              \<leadsto> (ufRestrict In Out\<cdot>(h (Abs_sbElem(inv convDiscrUp (sbHdElem\<cdot>sb)))) \<rightleftharpoons> (sbRt\<cdot>sb)))"
+"spfStep In Out \<equiv> \<Lambda> h. Abs_ufun (\<Lambda>  sb.  (ubDom\<cdot>sb = In) 
+                                              \<leadsto> (if (sbHdElemWell sb) then ufRestrict In Out\<cdot>(h (Abs_sbElem(inv convDiscrUp (sbHdElem\<cdot>sb)))) \<rightleftharpoons> (sbRt\<cdot>sb) else ubclLeast Out))"
 
 
-lemma spfStep_innerCont:"cont (\<lambda>  sb.  (ubDom\<cdot>sb = In \<and> sbHdElemWell sb) 
-                                              \<leadsto> (ufRestrict In Out\<cdot>(h (Abs_sbElem(inv convDiscrUp (sbHdElem\<cdot>sb)))) \<rightleftharpoons> (sbRt\<cdot>sb)))"
+lemma spfStep_innerMono:"monofun (\<lambda>  sb.  (ubDom\<cdot>sb = In) 
+                                              \<leadsto> (if (sbHdElemWell sb) then ufRestrict In Out\<cdot>(h (Abs_sbElem(inv convDiscrUp (sbHdElem\<cdot>sb)))) \<rightleftharpoons> (sbRt\<cdot>sb) else ubclLeast Out))"
+proof(rule monofunI)
+  fix x y::"'a stream\<^sup>\<Omega>"
+  assume a1:"x\<sqsubseteq>y"
+  have a2:"(ubDom\<cdot>x = In \<and> sbHdElemWell x) \<Longrightarrow> (ubDom\<cdot>y = In \<and> sbHdElemWell y)"
+    by (metis a1 below_bottom_iff sbHdElemWell_def ubdom_below ubgetch_below)
+  show "(ubDom\<cdot>x = In)\<leadsto>if sbHdElemWell x then ufRestrict In Out\<cdot>(h (Abs_sbElem (inv convDiscrUp (sbHdElem\<cdot>x)))) \<rightleftharpoons> sbRt\<cdot>x else ubclLeast Out \<sqsubseteq>
+       (ubDom\<cdot>y = In)\<leadsto>if sbHdElemWell y then ufRestrict In Out\<cdot>(h (Abs_sbElem (inv convDiscrUp (sbHdElem\<cdot>y)))) \<rightleftharpoons> sbRt\<cdot>y else ubclLeast Out"
+  proof(cases "ubDom\<cdot>x = In")
+    case True
+    then have true_x:"ubDom\<cdot>x = In"
+      by simp
+    then have true_y:"ubDom\<cdot>y = In"
+      using a1 ubdom_below by auto
+    then show ?thesis
+    proof(cases "sbHdElemWell x")
+      case True
+      have true_y2:"sbHdElemWell y"
+        using True a1 a2 true_y ubdom_below by auto
+      have a3:"sbHdElem\<cdot>x = sbHdElem\<cdot>y"
+        apply(rule sbHdElem_eq)
+        using True sbHdElemWell_def a1 by blast+
+      have "(ufRestrict In Out\<cdot>(h (Abs_sbElem (inv convDiscrUp (sbHdElem\<cdot>x)))) \<rightleftharpoons> sbRt\<cdot>x) \<sqsubseteq> (ufRestrict In Out\<cdot>(h (Abs_sbElem (inv convDiscrUp (sbHdElem\<cdot>y)))) \<rightleftharpoons> sbRt\<cdot>y)"
+        by (smt a1 a3 below_option_def po_eq_conv spfrt_step ufun_rel_eq)
+      then show ?thesis
+        by(simp add: True true_x true_y true_y2 some_below)
+    next
+      case False
+      then show ?thesis
+        by (smt a1 po_eq_conv sbrt_sbdom some_below ubclDom_ubundle_def ubcldom_least ubdom_below ufRestrict_dom ufRestrict_ran ufran_2_ubcldom2)
+    qed
+  next
+    case False
+    then show ?thesis
+      using a1 ubdom_below by force
+  qed
+qed
+  
+
+lemma spfStep_innerCont:"cont (\<lambda>  sb.  (ubDom\<cdot>sb = In) 
+                                              \<leadsto> (if (sbHdElemWell sb) then ufRestrict In Out\<cdot>(h (Abs_sbElem(inv convDiscrUp (sbHdElem\<cdot>sb)))) \<rightleftharpoons> (sbRt\<cdot>sb) else ubclLeast Out))"
   sorry
 
-lemma spfStep_innerWell:"ufWell (\<Lambda>  sb.  (ubDom\<cdot>sb = In \<and> sbHdElemWell sb) 
-                                              \<leadsto> (ufRestrict In Out\<cdot>(h (Abs_sbElem(inv convDiscrUp (sbHdElem\<cdot>sb)))) \<rightleftharpoons> (sbRt\<cdot>sb))) "
+lemma spfStep_innerWell:"ufWell (\<Lambda>  sb.  (ubDom\<cdot>sb = In) 
+                                              \<leadsto> (if (sbHdElemWell sb) then ufRestrict In Out\<cdot>(h (Abs_sbElem(inv convDiscrUp (sbHdElem\<cdot>sb)))) \<rightleftharpoons> (sbRt\<cdot>sb) else ubclLeast Out)) "
   sorry
 
 
 
-lemma spfStep_cont:"cont (\<lambda> h. Abs_ufun (\<Lambda>  sb.  (ubDom\<cdot>sb = In \<and> sbHdElemWell sb) 
-                                              \<leadsto> (ufRestrict In Out\<cdot>(h (Abs_sbElem(inv convDiscrUp (sbHdElem\<cdot>sb)))) \<rightleftharpoons> (sbRt\<cdot>sb))))"
+lemma spfStep_cont:"cont (\<lambda> h. Abs_ufun (\<Lambda>  sb.  (ubDom\<cdot>sb = In) 
+                                              \<leadsto> (if (sbHdElemWell sb) then ufRestrict In Out\<cdot>(h (Abs_sbElem(inv convDiscrUp (sbHdElem\<cdot>sb)))) \<rightleftharpoons> (sbRt\<cdot>sb) else ubclLeast Out)))"
   sorry
 
-lemma [simp]:"inj (\<lambda> h. Abs_ufun (\<Lambda>  sb.  (ubDom\<cdot>sb = In \<and> sbHdElemWell sb) 
-                                              \<leadsto> (ufRestrict In Out\<cdot>(h (Abs_sbElem(inv convDiscrUp (sbHdElem\<cdot>sb)))) \<rightleftharpoons> (sbRt\<cdot>sb))))" (*h must map to spf with dom = In and Range = Out and not map to ufLeast In Out*)
-proof(rule injI)
+lemma [simp]:"inj_on (\<lambda> h. Abs_ufun (\<Lambda>  sb.  (ubDom\<cdot>sb = In) 
+                                              \<leadsto> (if (sbHdElemWell sb) then ufRestrict In Out\<cdot>(h (Abs_sbElem(inv convDiscrUp (sbHdElem\<cdot>sb)))) \<rightleftharpoons> (sbRt\<cdot>sb) else ubclLeast Out))) {h. \<forall>m. ufDom\<cdot>(h m) = In \<and> ufRan\<cdot>(h m) = Out}" (*h must map to spf with dom = In and Range = Out and not map to ufLeast In Out*)
+proof(rule inj_onI)
   fix x y::"'a sbElem \<Rightarrow> ('a stream\<^sup>\<Omega>) ufun"
-  assume a1:" Abs_cufun (\<lambda>sb. (ubDom\<cdot>sb = In \<and> sbHdElemWell sb)\<leadsto>ufRestrict In Out\<cdot>(x (Abs_sbElem (inv convDiscrUp (sbHdElem\<cdot>sb)))) \<rightleftharpoons> sbRt\<cdot>sb) =
-              Abs_cufun (\<lambda>sb. (ubDom\<cdot>sb = In \<and> sbHdElemWell sb)\<leadsto>ufRestrict In Out\<cdot>(y (Abs_sbElem (inv convDiscrUp (sbHdElem\<cdot>sb)))) \<rightleftharpoons> sbRt\<cdot>sb)"
-  then have "\<forall>insb. Abs_cufun (\<lambda>sb. (ubDom\<cdot>sb = In \<and> sbHdElemWell sb)\<leadsto>ufRestrict In Out\<cdot>(x (Abs_sbElem (inv convDiscrUp (sbHdElem\<cdot>sb)))) \<rightleftharpoons> sbRt\<cdot>sb) \<rightleftharpoons> insb =
-              Abs_cufun (\<lambda>sb. (ubDom\<cdot>sb = In \<and> sbHdElemWell sb)\<leadsto>ufRestrict In Out\<cdot>(y (Abs_sbElem (inv convDiscrUp (sbHdElem\<cdot>sb)))) \<rightleftharpoons> sbRt\<cdot>sb) \<rightleftharpoons> insb"
-    by simp
-  then have a2:"\<forall> insb. (\<lambda>sb. (ubDom\<cdot>sb = In \<and> sbHdElemWell sb)\<leadsto>ufRestrict In Out\<cdot>(x (Abs_sbElem (inv convDiscrUp (sbHdElem\<cdot>sb)))) \<rightleftharpoons> sbRt\<cdot>sb) insb =
-           (\<lambda>sb. (ubDom\<cdot>sb = In \<and> sbHdElemWell sb)\<leadsto>ufRestrict In Out\<cdot>(y (Abs_sbElem (inv convDiscrUp (sbHdElem\<cdot>sb)))) \<rightleftharpoons> sbRt\<cdot>sb) insb"
-    apply(simp add: spfStep_innerWell spfStep_innerCont)
-    by (smt ufRestrict_dom ufapplyin_eq_pre)
-  have "(\<forall>elem. (x elem) \<noteq> ufLeast In Out \<and> ufDom\<cdot>(x elem) = In \<and> ufRan\<cdot>(x elem) = Out)"
-    sorry
-  then have "(\<lambda>sb. (ubDom\<cdot>sb = In \<and> sbHdElemWell sb)\<leadsto>ufRestrict In Out\<cdot>(x (Abs_sbElem (inv convDiscrUp (sbHdElem\<cdot>sb)))) \<rightleftharpoons> sbRt\<cdot>sb) =
-             (\<lambda>sb. (ubDom\<cdot>sb = In \<and> sbHdElemWell sb)\<leadsto>(x (Abs_sbElem (inv convDiscrUp (sbHdElem\<cdot>sb)))) \<rightleftharpoons> sbRt\<cdot>sb)"
-    by auto
-  moreover have "(\<lambda>sb. (ubDom\<cdot>sb = In \<and> sbHdElemWell sb)\<leadsto>ufRestrict In Out\<cdot>(y (Abs_sbElem (inv convDiscrUp (sbHdElem\<cdot>sb)))) \<rightleftharpoons> sbRt\<cdot>sb) =
-                 (\<lambda>sb. (ubDom\<cdot>sb = In \<and> sbHdElemWell sb)\<leadsto>(y (Abs_sbElem (inv convDiscrUp (sbHdElem\<cdot>sb)))) \<rightleftharpoons> sbRt\<cdot>sb)"
-    sorry
-  ultimately have "(\<lambda>sb. (ubDom\<cdot>sb = In \<and> sbHdElemWell sb)\<leadsto>(x (Abs_sbElem (inv convDiscrUp (sbHdElem\<cdot>sb)))) \<rightleftharpoons> sbRt\<cdot>sb) = 
-                   (\<lambda>sb. (ubDom\<cdot>sb = In \<and> sbHdElemWell sb)\<leadsto>(y (Abs_sbElem (inv convDiscrUp (sbHdElem\<cdot>sb)))) \<rightleftharpoons> sbRt\<cdot>sb)"
-    sorry
-  then show "x = y"
+  assume ax:"x \<in> {h::'a sbElem \<Rightarrow> ('a stream\<^sup>\<Omega>) ufun. \<forall>m::'a sbElem. ufDom\<cdot>(h m) = In \<and> ufRan\<cdot>(h m) = Out }"
+  assume ay:"y \<in> {h::'a sbElem \<Rightarrow> ('a stream\<^sup>\<Omega>) ufun. \<forall>m::'a sbElem. ufDom\<cdot>(h m) = In \<and> ufRan\<cdot>(h m) = Out}"
+  assume a1:" Abs_cufun (\<lambda>sb::'a stream\<^sup>\<Omega>. (ubDom\<cdot>sb = In)\<leadsto>if sbHdElemWell sb then ufRestrict In Out\<cdot>(x (Abs_sbElem (inv convDiscrUp (sbHdElem\<cdot>sb)))) \<rightleftharpoons> sbRt\<cdot>sb else ubclLeast Out) =
+       Abs_cufun (\<lambda>sb::'a stream\<^sup>\<Omega>. (ubDom\<cdot>sb = In)\<leadsto>if sbHdElemWell sb then ufRestrict In Out\<cdot>(y (Abs_sbElem (inv convDiscrUp (sbHdElem\<cdot>sb)))) \<rightleftharpoons> sbRt\<cdot>sb else ubclLeast Out)"
+  have ya:"(\<forall>elem.  ufDom\<cdot>(y elem) = In \<and> ufRan\<cdot>(y elem) = Out)"
+    using ay by auto
+  show "x = y"
     sorry
 qed
 
 lemma spfStep_inj:"inj (Rep_cfun(spfStep In Out))"  
-  by(simp add: spfStep_def spfStep_cont)
+  sorry
 
-lemma spfstep_insert: "spfStep In Out\<cdot>h= Abs_ufun (\<Lambda>  sb.  (ubDom\<cdot>sb = In \<and> sbHdElemWell sb) 
-                                              \<leadsto> (ufRestrict In Out\<cdot>(h (Abs_sbElem(inv convDiscrUp (sbHdElem\<cdot>sb)))) \<rightleftharpoons> (sbRt\<cdot>sb)))"
+lemma spfstep_insert: "spfStep In Out\<cdot>h= Abs_ufun (\<Lambda>  sb.  (ubDom\<cdot>sb = In) 
+                                              \<leadsto> (if (sbHdElemWell sb) then ufRestrict In Out\<cdot>(h (Abs_sbElem(inv convDiscrUp (sbHdElem\<cdot>sb)))) \<rightleftharpoons> (sbRt\<cdot>sb) else ubclLeast Out))"
   by(simp add: spfStep_def spfStep_cont)
 
 lemma spfstep_dom[simp]:s"ufDom\<cdot>(spfStep cIn cOut\<cdot>f) = cIn"
